theories/ftlr/ftlr_base.v
@@ -24,7 +24,7 @@ Section fundamental.
     → decodeInstrW w = i
     -> □ ▷ (∀ a0 a1 a2 a3 a4 w,
              full_map a0
-          -∗ (∀ (r1 : RegName) v, ⌜r1 ≠ PC⌝ → ⌜a0 !! r1 = Some v⌝ → (fixpoint interp1) v)
+          -∗ (∀ (r1 : RegName) v, ⌜r1 ≠ PC⌝ → ⌜r1 ≠ idc⌝ → ⌜a0 !! r1 = Some v⌝ → (fixpoint interp1) v)
           -∗ registers_mapsto (<[idc:=w]>(<[PC:=WCap a1 a2 a3 a4]> a0))
           -∗ na_own logrel_nais ⊤
              -∗ □ (fixpoint interp1) (WCap a1 a2 a3 a4) -∗ interp_conf)
